@prefix : <http://www.semanticweb.org/narrative-domain-application#> .
@prefix owl: <http://www.w3.org/2002/07/owl#> .
@prefix rdf: <http://www.w3.org/1999/02/22-rdf-syntax-ns#> .
@prefix xml: <http://www.w3.org/XML/1998/namespace> .
@prefix xsd: <http://www.w3.org/2001/XMLSchema#> .
@prefix rdfs: <http://www.w3.org/2000/01/rdf-schema#> .
@base <http://www.semanticweb.org/narrative-domain-application> .

<http://www.semanticweb.org/narrative-domain-application> rdf:type owl:Ontology .

#################################################################
#    Object Properties
#################################################################

###  http://www.semanticweb.org/narrative-domain-application#hasComponent
:hasComponent rdf:type owl:ObjectProperty ;
              owl:inverseOf :isComponentOf ;
              rdf:type owl:TransitiveProperty ;
              rdfs:comment "has Component is super property of: has Narrative and has Event."@en ;
              rdfs:label "has Component"@en .


###  http://www.semanticweb.org/narrative-domain-application#hasContractWith
:hasContractWith rdf:type owl:ObjectProperty ;
                 owl:inverseOf :makeContractWith ;
                 rdfs:domain :Narrator ;
                 rdfs:range :Publisher ;
                 owl:propertyChainAxiom ( :hasCreated
                                          :isNarrativeOf
                                          :hasPublisher
                                        ) ;
                 rdfs:comment "has Contract with relates a narrator to the publishers with whom it has a contract."@en ;
                 rdfs:label "has Contract With"@en .


###  http://www.semanticweb.org/narrative-domain-application#hasCreated
:hasCreated rdf:type owl:ObjectProperty ;
            owl:inverseOf :isCreatedBy ;
            rdfs:domain :Narrator ;
            rdfs:range :Narrative ;
            rdfs:comment "has Created relates a narrators to the narrative he has created."@en ;
            rdfs:label "has Created"@en .


###  http://www.semanticweb.org/narrative-domain-application#hasEvent
:hasEvent rdf:type owl:ObjectProperty ;
          rdfs:subPropertyOf :hasComponent ;
          owl:inverseOf :isEventOf ;
          rdf:type owl:InverseFunctionalProperty ;
          rdfs:domain :Narrative ;
          rdfs:range :Event ;
          owl:propertyDisjointWith :hasNarrative ;
          rdfs:comment "has Event is sub property of has Component and it relates a narrative to events that compose it."@en ;
          rdfs:label "has Event"@en .


###  http://www.semanticweb.org/narrative-domain-application#hasLocation
:hasLocation rdf:type owl:ObjectProperty ;
             owl:inverseOf :isLocationOf ;
             rdf:type owl:FunctionalProperty ;
             rdfs:domain :Event ;
             rdfs:range :Location ;
             rdfs:comment "has Location relates an event to a location where it occurs."@en ;
             rdfs:label "has Location"@en .


###  http://www.semanticweb.org/narrative-domain-application#hasNarrative
:hasNarrative rdf:type owl:ObjectProperty ;
              rdfs:subPropertyOf :hasComponent ;
              owl:inverseOf :isNarrativeOf ;
              rdf:type owl:InverseFunctionalProperty ;
              rdfs:domain :Book ;
              rdfs:range :Narrative ;
              rdfs:comment "has Narrative is sub property of has Component and it relates a book to narratives it reports."@en ;
              rdfs:label "has Narrative"@en .


###  http://www.semanticweb.org/narrative-domain-application#hasPartecipant
:hasPartecipant rdf:type owl:ObjectProperty ;
                owl:inverseOf :isPartecipantOf ;
                rdfs:comment "has Partecipant is super property of: has Partecipant Object and has Partecipant Character."@en ;
                rdfs:label "has Partecipant"@en .


###  http://www.semanticweb.org/narrative-domain-application#hasPartecipantCharacter
:hasPartecipantCharacter rdf:type owl:ObjectProperty ;
                         rdfs:subPropertyOf :hasPartecipant ;
                         owl:inverseOf :isPartecipantCharacterOf ;
                         rdfs:domain :Event ;
                         rdfs:range :Character ;
                         owl:propertyDisjointWith :hasPartecipantObject ;
                         rdfs:comment "has Partecipant Character is sub property of has Partecipant and it relates an events to character that partecipate in that event."@en ;
                         rdfs:label "has Partecipant Character"@en .


###  http://www.semanticweb.org/narrative-domain-application#hasPartecipantObject
:hasPartecipantObject rdf:type owl:ObjectProperty ;
                      rdfs:subPropertyOf :hasPartecipant ;
                      owl:inverseOf :isPartecipantObjectOf ;
                      rdfs:domain :Event ;
                      rdfs:range :Object ;
                      rdfs:comment "has Partecipant Object is sub property of has Partecipant and it relates an events to object that partecipate in that event."@en ;
                      rdfs:label "has Partecipant Object"@en .


###  http://www.semanticweb.org/narrative-domain-application#hasPublished
:hasPublished rdf:type owl:ObjectProperty ;
              owl:inverseOf :hasPublisher ;
              rdf:type owl:InverseFunctionalProperty ;
              rdfs:domain :Publisher ;
              rdfs:range :Book ;
              rdfs:comment "has Published relates a publisher to books it has published."@en ;
              rdfs:label "has Published"@en .


###  http://www.semanticweb.org/narrative-domain-application#hasPublisher
:hasPublisher rdf:type owl:ObjectProperty ,
                       owl:FunctionalProperty ;
              rdfs:domain :Book ;
              rdfs:range :Publisher ;
              rdfs:comment "has Publisher relates a books to the publishers who published it."@en ;
              rdfs:label "has Publisher"@en .


###  http://www.semanticweb.org/narrative-domain-application#isComponentOf
:isComponentOf rdf:type owl:ObjectProperty ,
                        owl:TransitiveProperty ;
               rdfs:comment "is Component Of is super property of: is Narrative Of and is Event Of."@en ;
               rdfs:label "is Component Of"@en .


###  http://www.semanticweb.org/narrative-domain-application#isCreatedBy
:isCreatedBy rdf:type owl:ObjectProperty ;
             rdfs:domain :Narrative ;
             rdfs:range :Narrator ;
             rdfs:comment "is Created By relates a narrative to narrators who has created it."@en ;
             rdfs:label "is Created By"@en .


###  http://www.semanticweb.org/narrative-domain-application#isEventOf
:isEventOf rdf:type owl:ObjectProperty ;
           rdfs:subPropertyOf :isComponentOf ;
           rdf:type owl:FunctionalProperty ;
           rdfs:domain :Event ;
           rdfs:range :Narrative ;
           owl:propertyDisjointWith :isNarrativeOf ;
           rdfs:comment "is Event  Of is sub property of is Component Of and it relates a event to the narratives it composes."@en ;
           rdfs:label "is Event Of"@en .


###  http://www.semanticweb.org/narrative-domain-application#isLocationOf
:isLocationOf rdf:type owl:ObjectProperty ,
                       owl:InverseFunctionalProperty ;
              rdfs:domain :Location ;
              rdfs:range :Event ;
              rdfs:comment "is Location Of relates a location to events occurring in that location."@en ;
              rdfs:label "is Location Of"@en .


###  http://www.semanticweb.org/narrative-domain-application#isNarrativeOf
:isNarrativeOf rdf:type owl:ObjectProperty ;
               rdfs:subPropertyOf :isComponentOf ;
               rdf:type owl:FunctionalProperty ;
               rdfs:domain :Narrative ;
               rdfs:range :Book ;
               rdfs:comment "is Narrative Of is sub property of is Component Of and it relates a narrative to the book that reports it."@en ;
               rdfs:label "is Narrative Of"@en .


###  http://www.semanticweb.org/narrative-domain-application#isPartecipantCharacterOf
:isPartecipantCharacterOf rdf:type owl:ObjectProperty ;
                          rdfs:subPropertyOf :isPartecipantOf ;
                          rdfs:domain :Character ;
                          rdfs:range :Event ;
                          owl:propertyDisjointWith :isPartecipantObjectOf ;
                          rdfs:comment "is Partecipant Character Of is sub property of is Partecipant Of and it relates a characters to events for which it is a partecipant."@en ;
                          rdfs:label "is Partecipant Character Of"@en .


###  http://www.semanticweb.org/narrative-domain-application#isPartecipantObjectOf
:isPartecipantObjectOf rdf:type owl:ObjectProperty ;
                       rdfs:subPropertyOf :isPartecipantOf ;
                       rdfs:domain :Object ;
                       rdfs:range :Event ;
                       rdfs:comment "is Partecipant Object Of is sub property of is Partecipant Of and it relates an object to events for which it is a partecipant."@en ;
                       rdfs:label "is Partecipant Object Of"@en .


###  http://www.semanticweb.org/narrative-domain-application#isPartecipantOf
:isPartecipantOf rdf:type owl:ObjectProperty ;
                 rdfs:comment "is Partecipant of is super property of: is Character Partecipant Of and is Object Partecipant Of."@en ;
                 rdfs:label "is Partecipant Of"@en .


###  http://www.semanticweb.org/narrative-domain-application#makeContractWith
:makeContractWith rdf:type owl:ObjectProperty ;
                  rdfs:domain :Publisher ;
                  rdfs:range :Narrator ;
                  rdfs:comment "make Contract With relates a publisher to narrators they have contracted with."@en ;
                  rdfs:label "make Contract With"@en .


#################################################################
#    Data properties
#################################################################

###  http://www.semanticweb.org/narrative-domain-application#hasCharacterName
:hasCharacterName rdf:type owl:DatatypeProperty ;
                  rdfs:subPropertyOf :hasName ;
                  rdf:type owl:FunctionalProperty ;
                  rdfs:domain :Character ;
                  rdfs:range xsd:string ;
                  owl:propertyDisjointWith :hasLocationName ,
                                           :hasObjectName ,
                                           :hasPublisherName ;
                  rdfs:comment "has Character Name relates a characters to its own name (represented as string)."@en ;
                  rdfs:label "has Character Name"@en .


###  http://www.semanticweb.org/narrative-domain-application#hasID
:hasID rdf:type owl:DatatypeProperty ,
                owl:FunctionalProperty ;
       rdfs:domain :Publisher ;
       rdfs:range xsd:positiveInteger ;
       owl:propertyDisjointWith :hasISBNCode ,
                                :hasName ,
                                :hasTitle ;
       rdfs:comment "has ID relates books with their own ID represented by positive integer."@en ;
       rdfs:label "has ID"@en .


###  http://www.semanticweb.org/narrative-domain-application#hasISBNCode
:hasISBNCode rdf:type owl:DatatypeProperty ,
                      owl:FunctionalProperty ;
             rdfs:domain :Book ;
             rdfs:range xsd:string ;
             owl:propertyDisjointWith :hasName ,
                                      :hasTitle ;
             rdfs:comment "has ISBN Code relates books with their own ISBN code represented by a string."@en ;
             rdfs:label "has ISBN Code"@en .


###  http://www.semanticweb.org/narrative-domain-application#hasLocationName
:hasLocationName rdf:type owl:DatatypeProperty ;
                 rdfs:subPropertyOf :hasName ;
                 rdf:type owl:FunctionalProperty ;
                 rdfs:domain :Location ;
                 rdfs:range xsd:string ;
                 owl:propertyDisjointWith :hasObjectName ,
                                          :hasPublisherName ;
                 rdfs:comment "has Location Name relates a location to its own name (represented as string)."@en ;
                 rdfs:label "has Location Name"@en .


###  http://www.semanticweb.org/narrative-domain-application#hasName
:hasName rdf:type owl:DatatypeProperty ;
         owl:propertyDisjointWith :hasTitle ;
         rdfs:comment "has Name relates individuals of a given class to their own name represented as string."@en ;
         rdfs:label "has Name"@en .


###  http://www.semanticweb.org/narrative-domain-application#hasObjectName
:hasObjectName rdf:type owl:DatatypeProperty ;
               rdfs:subPropertyOf :hasName ;
               rdf:type owl:FunctionalProperty ;
               rdfs:domain :Object ;
               rdfs:range xsd:string ;
               owl:propertyDisjointWith :hasPublisherName ;
               rdfs:comment "has Object Name relates an object to its own name (represented as string)."@en ;
               rdfs:label "has Object Name"@en .


###  http://www.semanticweb.org/narrative-domain-application#hasPublisherName
:hasPublisherName rdf:type owl:DatatypeProperty ;
                  rdfs:subPropertyOf :hasName ;
                  rdf:type owl:FunctionalProperty ;
                  rdfs:domain :Publisher ;
                  rdfs:range xsd:string ;
                  rdfs:comment "has Publisher Name relates a publisher to its own name (represented as string)."@en ;
                  rdfs:label "has Publisher Name"@en .


###  http://www.semanticweb.org/narrative-domain-application#hasTitle
:hasTitle rdf:type owl:DatatypeProperty ,
                   owl:FunctionalProperty ;
          rdfs:domain :Book ;
          rdfs:range xsd:string ;
          rdfs:comment "has Title relates books with their own title represented by a string."@en ;
          rdfs:label "has Title"@en .


#################################################################
#    Classes
#################################################################

###  http://www.semanticweb.org/narrative-domain-application#Book
:Book rdf:type owl:Class ;
      rdfs:subClassOf [ rdf:type owl:Restriction ;
                        owl:onProperty :hasNarrative ;
                        owl:minQualifiedCardinality "1"^^xsd:nonNegativeInteger ;
                        owl:onClass :Narrative
                      ] ,
                      [ rdf:type owl:Restriction ;
                        owl:onProperty :hasPublisher ;
                        owl:qualifiedCardinality "1"^^xsd:nonNegativeInteger ;
                        owl:onClass :Publisher
                      ] ,
                      [ rdf:type owl:Restriction ;
                        owl:onProperty :hasISBNCode ;
                        owl:qualifiedCardinality "1"^^xsd:nonNegativeInteger ;
                        owl:onDataRange xsd:string
                      ] ,
                      [ rdf:type owl:Restriction ;
                        owl:onProperty :hasTitle ;
                        owl:qualifiedCardinality "1"^^xsd:nonNegativeInteger ;
                        owl:onDataRange xsd:string
                      ] ;
      owl:disjointWith :Bookshop ,
                       :Character ,
                       :Event ,
                       :Location ,
                       :Narrative ,
                       :Narrator ,
                       :Object ,
                       :Publisher ;
      rdfs:comment "A book reports one or more narrative, it has a title and an ISBN code and has exactly one publisher."@en ;
      rdfs:label "Book"@en .


###  http://www.semanticweb.org/narrative-domain-application#Bookshop
:Bookshop rdf:type owl:Class ;
          owl:disjointWith :Character ,
                           :Event ,
                           :Location ,
                           :Narrative ,
                           :Narrator ,
                           :Object ,
                           :Publisher ;
          rdfs:comment "A bookshop is a shop that sells books."@en ;
          rdfs:label "Bookshop"@en .


###  http://www.semanticweb.org/narrative-domain-application#Character
:Character rdf:type owl:Class ;
           rdfs:subClassOf [ rdf:type owl:Restriction ;
                             owl:onProperty :hasCharacterName ;
                             owl:qualifiedCardinality "1"^^xsd:nonNegativeInteger ;
                             owl:onDataRange xsd:string
                           ] ;
           owl:disjointWith :Event ,
                            :Location ,
                            :Narrative ,
                            :Narrator ,
                            :Object ,
                            :Publisher ;
           owl:disjointUnionOf ( :Human
                                 :NotHuman
                               ) ;
           rdfs:comment "A character can be human or not human, it has a name and it partecipates to an event."@en ;
           rdfs:label "Character"@en .


###  http://www.semanticweb.org/narrative-domain-application#Event
:Event rdf:type owl:Class ;
       rdfs:subClassOf [ rdf:type owl:Restriction ;
                         owl:onProperty :hasPartecipantCharacter ;
                         owl:allValuesFrom :Character
                       ] ,
                       [ rdf:type owl:Restriction ;
                         owl:onProperty :hasPartecipantObject ;
                         owl:allValuesFrom :Object
                       ] ,
                       [ rdf:type owl:Restriction ;
                         owl:onProperty :hasPartecipant ;
                         owl:minQualifiedCardinality "1"^^xsd:nonNegativeInteger ;
                         owl:onClass [ rdf:type owl:Class ;
                                       owl:unionOf ( :Character
                                                     :Object
                                                   )
                                     ]
                       ] ,
                       [ rdf:type owl:Restriction ;
                         owl:onProperty :hasLocation ;
                         owl:qualifiedCardinality "1"^^xsd:nonNegativeInteger ;
                         owl:onClass :Location
                       ] ;
       owl:disjointWith :Location ,
                        :Narrative ,
                        :Narrator ,
                        :Object ,
                        :Publisher ;
       rdfs:comment "A event is narrative event that occur in exactlly one location."@en ;
       rdfs:label "Event"@en .


###  http://www.semanticweb.org/narrative-domain-application#FictionalLocation
:FictionalLocation rdf:type owl:Class ;
                   rdfs:subClassOf :Location ;
                   owl:disjointWith :RealLocation ;
                   rdfs:comment "A fictional location is a location used in event that is invented, not real."@en ;
                   rdfs:label "Fictional Location"@en .


###  http://www.semanticweb.org/narrative-domain-application#Human
:Human rdf:type owl:Class ;
       rdfs:subClassOf :Character ;
       owl:disjointWith :NotHuman ;
       rdfs:comment "A human character is character with human features."@en ;
       rdfs:label "Human Characters"@en .


###  http://www.semanticweb.org/narrative-domain-application#Location
:Location rdf:type owl:Class ;
          rdfs:subClassOf [ rdf:type owl:Restriction ;
                            owl:onProperty :hasLocationName ;
                            owl:qualifiedCardinality "1"^^xsd:nonNegativeInteger ;
                            owl:onDataRange xsd:string
                          ] ;
          owl:disjointWith :Narrative ,
                           :Narrator ,
                           :Object ,
                           :Publisher ;
          owl:disjointUnionOf ( :FictionalLocation
                                :RealLocation
                              ) ;
          rdfs:comment "A location can be real or fictional, it has a name and it is a place where a narrative event happens."@en ;
          rdfs:label "Location"@en .


###  http://www.semanticweb.org/narrative-domain-application#Narrative
:Narrative rdf:type owl:Class ;
           rdfs:subClassOf [ rdf:type owl:Restriction ;
                             owl:onProperty :hasEvent ;
                             owl:allValuesFrom :Event
                           ] ,
                           [ rdf:type owl:Restriction ;
                             owl:onProperty :hasEvent ;
                             owl:minQualifiedCardinality "1"^^xsd:nonNegativeInteger ;
                             owl:onClass :Event
                           ] ,
                           [ rdf:type owl:Restriction ;
                             owl:onProperty :isCreatedBy ;
                             owl:minQualifiedCardinality "1"^^xsd:nonNegativeInteger ;
                             owl:onClass :Narrator
                           ] ;
           owl:disjointWith :Narrator ,
                            :Object ,
                            :Publisher ;
           rdfs:comment "A narrative is composed (exclusive) of one or more event, it is created by a narrator and it is reported in a book."@en ;
           rdfs:label "Narrative"@en .


###  http://www.semanticweb.org/narrative-domain-application#Narrator
:Narrator rdf:type owl:Class ;
          rdfs:subClassOf [ rdf:type owl:Restriction ;
                            owl:onProperty :hasContractWith ;
                            owl:allValuesFrom :Publisher
                          ] ,
                          [ rdf:type owl:Restriction ;
                            owl:onProperty :hasContractWith ;
                            owl:minQualifiedCardinality "1"^^xsd:nonNegativeInteger ;
                            owl:onClass :Publisher
                          ] ;
          owl:disjointWith :Object ,
                           :Publisher ;
          rdfs:comment "A narrator creates narratives and has at least one contract with a publisher."@en ;
          rdfs:label "Narrator"@en .


###  http://www.semanticweb.org/narrative-domain-application#NotHuman
:NotHuman rdf:type owl:Class ;
          rdfs:subClassOf :Character ;
          rdfs:comment "A not human character is a character with non-human features."@en ;
          rdfs:label "Not Human Characters"@en .


###  http://www.semanticweb.org/narrative-domain-application#Object
:Object rdf:type owl:Class ;
        rdfs:subClassOf [ rdf:type owl:Restriction ;
                          owl:onProperty :hasObjectName ;
                          owl:qualifiedCardinality "1"^^xsd:nonNegativeInteger ;
                          owl:onDataRange xsd:string
                        ] ;
        owl:disjointWith :Publisher ;
        rdfs:comment "An object has a name and partecipated into an event."@en ;
        rdfs:label "Object"@en .


###  http://www.semanticweb.org/narrative-domain-application#Organization
:Organization rdf:type owl:Class ;
              rdfs:comment "An organization (example: Publisher is an organization)."@en ;
              rdfs:label "Organization"@en .


###  http://www.semanticweb.org/narrative-domain-application#Publisher
:Publisher rdf:type owl:Class ;
           rdfs:subClassOf :Organization ,
                           [ rdf:type owl:Restriction ;
                             owl:onProperty :hasPublished ;
                             owl:someValuesFrom :Book
                           ] ,
                           [ rdf:type owl:Restriction ;
                             owl:onProperty :hasPublished ;
                             owl:minQualifiedCardinality "2"^^xsd:nonNegativeInteger ;
                             owl:onClass :Book
                           ] ,
                           [ rdf:type owl:Restriction ;
                             owl:onProperty :hasID ;
                             owl:qualifiedCardinality "1"^^xsd:nonNegativeInteger ;
                             owl:onDataRange xsd:positiveInteger
                           ] ,
                           [ rdf:type owl:Restriction ;
                             owl:onProperty :hasPublisherName ;
                             owl:qualifiedCardinality "1"^^xsd:nonNegativeInteger ;
                             owl:onDataRange xsd:string
                           ] ;
           rdfs:comment "A publisher is an organization identified by a name and an ID, it publishes more then one book and it makes contract with some narrators."@en ;
           rdfs:label "Publisher"@en .


###  http://www.semanticweb.org/narrative-domain-application#RealLocation
:RealLocation rdf:type owl:Class ;
              rdfs:subClassOf :Location ;
              rdfs:comment "A real location is a location used in event that is real, not invented."@en ;
              rdfs:label "Real Location"@en .


#################################################################
#    Individuals
#################################################################

###  http://www.semanticweb.org/narrative-domain-application#CaptainHook
:CaptainHook rdf:type owl:NamedIndividual ,
                      :Human ;
             :isPartecipantCharacterOf :PeterPanDefeatsCaptainHook ;
             :hasCharacterName "Captain Hook"^^xsd:string ;
             rdfs:label "Captain Hook"@en .


###  http://www.semanticweb.org/narrative-domain-application#DisneyHistory
:DisneyHistory rdf:type owl:NamedIndividual ,
                        :Book ;
               :hasNarrative :PeterPanHistory ,
                             :PocahontasHistory ;
               :hasPublisher :Feltrinelli ;
               :hasISBNCode "1010"^^xsd:string ;
               :hasTitle "Disney History"^^xsd:string ;
               rdfs:label "Disney History"@en .


###  http://www.semanticweb.org/narrative-domain-application#FakeDeathOfMattiaPascal
:FakeDeathOfMattiaPascal rdf:type owl:NamedIndividual ,
                                  :Event ;
                         :hasLocation :Italy ;
                         :hasPartecipantCharacter :MattiaPascal ;
                         :isEventOf :NarrativeOfMattiaPascal ;
                         rdfs:label "Fake death of Mattia Pascal" .


###  http://www.semanticweb.org/narrative-domain-application#Feltrinelli
:Feltrinelli rdf:type owl:NamedIndividual ,
                      :Publisher ;
             :makeContractWith :MarioRossi ;
             :hasID "200"^^xsd:positiveInteger ;
             :hasPublisherName "Feltrinelli"^^xsd:string .


###  http://www.semanticweb.org/narrative-domain-application#FeltrinelliPisa
:FeltrinelliPisa rdf:type owl:NamedIndividual ,
                          :Bookshop .


###  http://www.semanticweb.org/narrative-domain-application#GiovanniVerdi
:GiovanniVerdi rdf:type owl:NamedIndividual ,
                        :Narrator ;
               :hasContractWith :Feltrinelli ;
               :hasCreated :PeterPanHistory .


###  http://www.semanticweb.org/narrative-domain-application#Hook
:Hook rdf:type owl:NamedIndividual ,
               :Object ;
      :hasObjectName "Hook"^^xsd:string .


###  http://www.semanticweb.org/narrative-domain-application#IlFuMattiaPascal
:IlFuMattiaPascal rdf:type owl:NamedIndividual ,
                           :Book ;
                  :hasNarrative :NarrativeOfMattiaPascal ;
                  :hasPublisher :Mondadori ;
                  :hasISBNCode "2020"^^xsd:string ;
                  :hasTitle "Il fu Mattia Pascal"^^xsd:string ;
                  rdfs:label "Il fu Mattia Pascal"^^xsd:string .


###  http://www.semanticweb.org/narrative-domain-application#Italy
:Italy rdf:type owl:NamedIndividual ,
                :RealLocation ;
       :isLocationOf :FakeDeathOfMattiaPascal ;
       :hasLocationName "Italy"^^xsd:string .


###  http://www.semanticweb.org/narrative-domain-application#JohnSmith
:JohnSmith rdf:type owl:NamedIndividual ,
                    :Human ;
           :isPartecipantCharacterOf :PocahontasMeetJohnSmith ;
           :hasCharacterName "John Smith"^^xsd:string .


###  http://www.semanticweb.org/narrative-domain-application#London
:London rdf:type owl:NamedIndividual ,
                 :RealLocation ;
        :hasLocationName "London"^^xsd:string .


###  http://www.semanticweb.org/narrative-domain-application#LuigiPirandello
:LuigiPirandello rdf:type owl:NamedIndividual ,
                          :Narrator ;
                 :hasCreated :NarrativeOfMattiaPascal .


###  http://www.semanticweb.org/narrative-domain-application#MagicPowder
:MagicPowder rdf:type owl:NamedIndividual ,
                      :Object ;
             :isPartecipantObjectOf :TrilliCreateMagicPowder ;
             :hasObjectName "Magic Powder"^^xsd:string .


###  http://www.semanticweb.org/narrative-domain-application#MarioRossi
:MarioRossi rdf:type owl:NamedIndividual ,
                     :Narrator ;
            :hasCreated :PocahontasHistory .


###  http://www.semanticweb.org/narrative-domain-application#MattiaPascal
:MattiaPascal rdf:type owl:NamedIndividual ,
                       :Human ;
              :isPartecipantCharacterOf :FakeDeathOfMattiaPascal ;
              :hasCharacterName "Mattia Pascal"^^xsd:string .


###  http://www.semanticweb.org/narrative-domain-application#Mondadori
:Mondadori rdf:type owl:NamedIndividual ,
                    :Publisher ;
           :hasPublished :IlFuMattiaPascal ;
           :makeContractWith :LuigiPirandello ;
           :hasID "300"^^xsd:positiveInteger ;
           :hasPublisherName "Mondadori"^^xsd:string .


###  http://www.semanticweb.org/narrative-domain-application#NarrativeOfMattiaPascal
:NarrativeOfMattiaPascal rdf:type owl:NamedIndividual ,
                                  :Narrative ;
                         :hasEvent :FakeDeathOfMattiaPascal ;
                         :isCreatedBy :LuigiPirandello ;
                         :isNarrativeOf :IlFuMattiaPascal .


###  http://www.semanticweb.org/narrative-domain-application#Neverland
:Neverland rdf:type owl:NamedIndividual ,
                    :FictionalLocation ;
           :isLocationOf :PeterPanDefeatsCaptainHook ;
           :hasLocationName "Neverland"^^xsd:string .


###  http://www.semanticweb.org/narrative-domain-application#PeterPan
:PeterPan rdf:type owl:NamedIndividual ,
                   :Human ;
          :isPartecipantCharacterOf :PeterPanMeetWendy ;
          :hasCharacterName "Peter Pan"^^xsd:string .


###  http://www.semanticweb.org/narrative-domain-application#PeterPanDefeatsCaptainHook
:PeterPanDefeatsCaptainHook rdf:type owl:NamedIndividual ,
                                     :Event ;
                            :hasLocation :Neverland ;
                            :hasPartecipantCharacter :CaptainHook ,
                                                     :PeterPan ;
                            :hasPartecipantObject :Hook ;
                            :isEventOf :PeterPanHistory ;
                            rdfs:label "Peter Pan Defeats Captain Hook" .


###  http://www.semanticweb.org/narrative-domain-application#PeterPanHistory
:PeterPanHistory rdf:type owl:NamedIndividual ,
                          :Narrative ;
                 :hasEvent :PeterPanMeetWendy ,
                           :TrilliCreateMagicPowder ;
                 :isCreatedBy :GiovanniVerdi .


###  http://www.semanticweb.org/narrative-domain-application#PeterPanMeetWendy
:PeterPanMeetWendy rdf:type owl:NamedIndividual ,
                            :Event ;
                   :hasLocation :London ;
                   :hasPartecipantCharacter :PeterPan ,
                                            :Wendy ;
                   :isEventOf :PeterPanHistory ;
                   rdfs:label "Peter Pan Meets Wendy" .


###  http://www.semanticweb.org/narrative-domain-application#Pocahontas
:Pocahontas rdf:type owl:NamedIndividual ,
                     :Human ;
            :isPartecipantCharacterOf :PocahontasMeetJohnSmith ;
            :hasCharacterName "Pocahontas"^^xsd:string .


###  http://www.semanticweb.org/narrative-domain-application#PocahontasHistory
:PocahontasHistory rdf:type owl:NamedIndividual ,
                            :Narrative ;
                   :hasEvent :PocahontasMeetJohnSmith ;
                   :isNarrativeOf :DisneyHistory .


###  http://www.semanticweb.org/narrative-domain-application#PocahontasMeetJohnSmith
:PocahontasMeetJohnSmith rdf:type owl:NamedIndividual ,
                                  :Event ;
                         :hasLocation :Virginia ;
                         :hasPartecipantCharacter :JohnSmith ,
                                                  :Pocahontas ;
                         :isEventOf :PocahontasHistory ;
                         rdfs:label "Pochaontas meets John Smith" .


###  http://www.semanticweb.org/narrative-domain-application#Trilli
:Trilli rdf:type owl:NamedIndividual ,
                 :NotHuman ;
        :isPartecipantCharacterOf :TrilliCreateMagicPowder ;
        :hasCharacterName "Trilli"^^xsd:string .


###  http://www.semanticweb.org/narrative-domain-application#TrilliCreateMagicPowder
:TrilliCreateMagicPowder rdf:type owl:NamedIndividual ,
                                  :Event ;
                         :hasLocation :Neverland ;
                         :hasPartecipantCharacter :Trilli ;
                         :hasPartecipantObject :MagicPowder ;
                         rdfs:label "Trilli create magic powder" .


###  http://www.semanticweb.org/narrative-domain-application#Virginia
:Virginia rdf:type owl:NamedIndividual ,
                   :RealLocation ;
          :isLocationOf :PocahontasMeetJohnSmith ;
          :hasLocationName "Virginia"^^xsd:string ;
          rdfs:label "Virginia (America)"@en .


###  http://www.semanticweb.org/narrative-domain-application#Wendy
:Wendy rdf:type owl:NamedIndividual ,
                :Human ;
       :isPartecipantCharacterOf :PeterPanMeetWendy ;
       :hasCharacterName "Wendy"^^xsd:string .


###  Generated by the OWL API (version 4.5.9.2019-02-01T07:24:44Z) https://github.com/owlcs/owlapi
